theories/Indexed/FunctionFacts.v
@@ -1,0 +1,15 @@
+From Coq Require Import
+     Setoid
+     Morphisms.
+
+From ITree Require Import
+     Indexed.Function
+     Indexed.Relation.
+
+Instance Proper_apply_IFun {E F : Type -> Type} {T : Type}
+         (RE : forall T, E T -> E T -> Prop)
+         (RF : forall T, F T -> F T -> Prop)
+  : Proper (i_respectful RE RF ==> RE T ==> RF T) apply_IFun.
+Proof.
+  repeat red; eauto.
+Qed.
